x86/RelocProgSemantics3.v
@@ -24,7 +24,7 @@ Context `{external_calls_prf: ExternalCalls}.
 
 Definition decode_tables (p:program) : res program :=
   match prog_sectable p with
-    snull :: sdata :: scode :: strsec :: symsec :: datarelocsec :: coderelocsec :: shstrsec :: nil =>
+    sdata :: scode :: strsec :: symsec :: datarelocsec :: coderelocsec :: shstrsec :: nil =>
     do ds <- decode_reloctable_section datarelocsec;
       do cs <- decode_reloctable_section coderelocsec;
       do (symbs, strmap) <- decode_strtable_section strsec;
@@ -33,13 +33,13 @@ Definition decode_tables (p:program) : res program :=
           prog_defs := prog_defs p;
           prog_public := prog_public p;
           prog_main := prog_main p;
-          prog_sectable := [snull; sdata; scode];
+          prog_sectable := [sdata; scode];
           prog_symbtable := syms;
           prog_strtable := PTree.empty Z;
           prog_reloctables := {| reloctable_code := cs; reloctable_data := ds |};
           prog_senv := prog_senv p;
         |}
-  | _ => Error (msg "Expected 8 sections [null,data,code,str,symb,reldata,relcode,shstr]")
+  | _ => Error (msg "Expected 7 sections [data,code,str,symb,reldata,relcode,shstr]")
   end.
 
 Inductive initial_state (prog: program) (rs: regset) (s: state): Prop :=
